fixed confluence proof for current lean version

Lambda.lean
@@ -8,7 +8,7 @@
 
 
 open Fin
-open Option
+-- open Option
 
 inductive Context : Type
 | zero : Context
@@ -72,16 +72,16 @@ def subLast {n} (t1 : Term (succ n)) (t2 : Term n) : Term n :=
   subst (substZero t2) t1
 
 mutual
-  inductive Neutral : ∀{Γ}, Term Γ → Type
+  inductive Neutral : ∀{Γ}, Term Γ → Prop
   | var : ∀{Γ}, (x : Var Γ) → Neutral (var x)
   | app : ∀{Γ}, {t1 t2 : Term Γ} → Neutral t1 → Normal t2 → Neutral (app t1 t2)
 
-  inductive Normal : ∀{Γ}, Term Γ → Type
+  inductive Normal : ∀{Γ}, Term Γ → Prop
   | neu : ∀{Γ}, {t : Term Γ} → Neutral t → Normal t
   | lam : ∀{Γ}, {t : Term (succ Γ)} → Normal t → Normal (lam t)
 end
 
-inductive Step : ∀{Γ}, Term Γ → Term Γ → Type where
+inductive Step : ∀{Γ}, Term Γ → Term Γ → Prop where
 | app1 : ∀ {Γ} {L L' M : Term Γ},
     Step L L'
     → Step (app L M) (app L' M)
@@ -102,33 +102,6 @@ inductive MultiStep : ∀ {Γ}, Term Γ → Term Γ → Type
 | halt : ∀ {Γ} {t : Term Γ}, MultiStep t t
 | step : ∀ {Γ} {t1 t2 t3 : Term Γ},
   Step t1 t2 → MultiStep t2 t3 → MultiStep t1 t3
-
-def progress {Γ} (M : Term Γ)
-  : (Σ N, Step M N) ⊕ (Normal M)
-  := match M with
-     | (var x) => Sum.inr (Normal.neu (Neutral.var x))
-     | lam N => match progress N with
-                | Sum.inl ⟨_ , s⟩ => Sum.inl ⟨_ , Step.lam s⟩
-                | Sum.inr t => Sum.inr (Normal.lam t)
-     | (app (lam _) _) => Sum.inl ⟨_ , Step.beta⟩
-     | (app (var x) M) => match progress M with
-              | Sum.inl ⟨_ , s⟩ => Sum.inl ⟨_ , Step.app2 s⟩
-              | Sum.inr normN => Sum.inr (Normal.neu (Neutral.app (Neutral.var x) normN))
-     | (app (app a b) M) => match progress (app a b) with
-              | Sum.inl ⟨_ , s⟩ => Sum.inl ⟨_ , Step.app1 s⟩
-              | Sum.inr (Normal.neu normN) => match progress M with
-                    | Sum.inl ⟨_ , s⟩ => Sum.inl  ⟨_ , Step.app2 s⟩
-                    | Sum.inr normM => Sum.inr (Normal.neu (Neutral.app normN normM))
-
-def eval {Γ} (fuel : Nat) (t1 : Term Γ)
-  : Option (Σ t2, ((MultiStep t1 t2) × (Normal t2))) :=
-  match fuel with
-  | Nat.zero => none
-  | Nat.succ fuel' => match progress t1 with
-    | Sum.inl ⟨t' , s⟩ => do
-        let ⟨final , steps , nf⟩ <- eval fuel' t'
-        some ⟨final , MultiStep.step s steps , nf⟩
-    | Sum.inr norm => some ⟨t1 , MultiStep.halt , norm⟩
 
 -- infix:50 " ~>> " => MultiStep
 -- infix:50 " ~>> " => MultiStep
@@ -287,7 +260,7 @@ theorem composeRename {n1} {M : Term n1}
 -- It seems that lean can't simp by locally defined definitions?
 def ren' {ren : {Γ : Context} → Ren Γ (Context.succ Γ)}
   : ∀{Γ}, Ren Γ (succ Γ) := fun {Γ} => match Γ with
-  | Context.zero => fun y => False.rec (noVarZero y)
+  | Context.zero => fun y => False.rec _ (noVarZero y)
   | Context.succ _x' => ext ren
 
 theorem commuteSubstRename {Γ} {M : Term Γ}
@@ -328,8 +301,7 @@ theorem extsSeq {Γ Δ Δ'} {sub1 : Subst Γ Δ} {sub2 : Subst Δ Δ'}
     simp [compose]
     simp [exts]
     rw [<- commuteSubstRename]
-    . rfl
-    . intro x; rfl
+    simp [exts]
 
 theorem subSub {n1} {M : Term n1}
   : ∀ {n2 n3} {sub1 : Subst n1 n2} {sub2 : Subst n2 n3},
@@ -414,7 +386,7 @@ theorem renameSubstCommute {Γ Δ} {N : Term (succ Γ)} {M : Term Γ} {ren : Ren
 ---------- A proof of confluence -----------------------------------------------
 --------------------------------------------------------------------------------
 
-inductive Par : ∀{Γ}, Term Γ → Term Γ → Type
+inductive Par : ∀{Γ}, Term Γ → Term Γ → Prop
 | pvar : ∀{Γ} {x : Var Γ}, Par (var x) (var x)
 | plam : ∀{Γ} {N N' : Term (succ Γ)},
   Par N N' → Par (lam N) (lam N')
@@ -423,7 +395,7 @@ inductive Par : ∀{Γ}, Term Γ → Term Γ → Type
 | pbeta : ∀{Γ}{N N' : Term (succ Γ)} {M M' : Term Γ},
   Par N N' → Par M M' → Par (app (lam N) M) (subLast N' M')
 
-def ParSubst {Γ} {Δ} (sub1 sub2 : Subst Γ Δ) : Type :=
+def ParSubst {Γ} {Δ} (sub1 sub2 : Subst Γ Δ) : Prop :=
   {x : Var Γ} → Par (sub1 x) (sub2 x)
 
 theorem parRename {Γ} {M M' : Term Γ}
@@ -496,7 +468,7 @@ theorem parRefl {Γ} {M : Term Γ} : Par M M := by
 -- since the eta rule involves a substiution
 theorem parDiamond {Γ} {t t1 t2 : Term Γ}
   (p1 : Par t t1) (p2 : Par t t2)
-  : Σ t', Par t1 t' × Par t2 t' :=
+  : ∃ t', Par t1 t' ∧ Par t2 t' :=
   match p1, p2 with
   | Par.pvar, Par.pvar => ⟨_, Par.pvar, Par.pvar⟩
   | Par.papp a1 b1, Par.papp a2 b2 =>
@@ -522,23 +494,23 @@ theorem parDiamond {Γ} {t t1 t2 : Term Γ}
 --------------------------------------------------------------------------------
 --------------------------------------------------------------------------------
 -------- Relations - from Nipkow (2001)
-def Relation (A : Type) : Type 1 := A → A → Type
+def Relation (A : Type) : Type := A → A → Prop
 
 inductive Proof (P : Prop) : Type
 | proof : P → Proof P
 
 def closeRef {A} (R : Relation A) : Relation A :=
-  fun x y => (Proof (x = y)) ⊕ R x y
+  fun x y => x = y ∨ R x y
 
 def liftRef {A} {B} {R : Relation A} {R' : Relation B} {x y : A} (f : A → B)
   (ctr : ∀{x y}, R x y → R' (f x) (f y))
   : closeRef R x y → closeRef R' (f x) (f y) :=
   fun s => match s with
-  | Sum.inl (Proof.proof rfl) => Sum.inl (Proof.proof rfl)
-  | Sum.inr s' => Sum.inr (ctr s')
+  | Or.inl rfl => Or.inl rfl
+  | Or.inr s' => Or.inr (ctr s')
 
 -- transitive relflexive closure of a relation
-inductive closure {A} (R : Relation A) : A → A → Type
+inductive closure {A} (R : Relation A) : A → A → Prop
 | refl : ∀{a : A}, closure R a a
 | cons : ∀{x y : A}, R x y → closure R y z  → closure R x z
 
@@ -559,7 +531,7 @@ def liftCsr {A} {B} {R : Relation A} {R' : Relation B} {x y : A} (f : A → B)
   | closure.refl => closure.refl
   | closure.cons xy yz => closure.cons (ctr xy) (liftCsr f ctr yz)
 
-inductive union {A} (R S : Relation A) : A → A → Type
+inductive union {A} (R S : Relation A) : A → A → Prop
 | r : ∀{x y}, R x y → union R S x y
 | s : ∀{x y}, S x y → union R S x y
 
@@ -596,12 +568,12 @@ def unionClosureToClosureUnion {A x y} {R S : Relation A}
   | union.s s => rightClosureUnion s
 
 -- All from Nipkow paper
-def square {A} (R S T U : Relation A) : Type :=
-  {x y z : A} → R x y → S x z → Σ u, T y u × U z u
+def square {A} (R S T U : Relation A) : Prop :=
+  {x y z : A} → R x y → S x z → ∃ u, T y u ∧ U z u
 
-def commute {A} (R S : Relation A) : Type := square R S S R
-def diamond {A} (R : Relation A) : Type := commute R R
-def confluent {A} (R : Relation A) : Type := diamond (closure R)
+def commute {A} (R S : Relation A) : Prop := square R S S R
+def diamond {A} (R : Relation A) : Prop := commute R R
+def confluent {A} (R : Relation A) : Prop := diamond (closure R)
 
 --     x --R-- y
 --     |       |
@@ -618,9 +590,9 @@ theorem stripLemma {A} {R S : Relation A}
   | closure.cons xx' x'z =>
     let ⟨out, s, r⟩ := sq Rxy xx'
     match r with
-    | Sum.inl (Proof.proof p) =>
+    | Or.inl p =>
       ⟨z, transitivity s (by rw [<- p]; exact x'z), closure.refl⟩
-    | Sum.inr r' =>
+    | Or.inr r' =>
       let ⟨out2, s2, r2⟩ := stripLemma sq r' x'z
       ⟨out2, transitivity s s2, r2⟩
 
@@ -684,7 +656,7 @@ def renFree {Γ1 Γ2} (ren : Ren Γ1 Γ2) (t : Term Γ2) : Prop :=
 
 def zFree {Γ} (t : Term (succ Γ)) : Prop := renFree Var.succ t
 
-inductive StepEta : ∀{Γ}, Term Γ → Term Γ → Type where
+inductive StepEta : ∀{Γ}, Term Γ → Term Γ → Prop where
 | app1 : ∀ {Γ} {L L' M : Term Γ},
     StepEta L L'
     → StepEta (app L M) (app L' M)
@@ -729,7 +701,7 @@ theorem etaRename {Γ} {M M' : Term Γ}
 
 --------------
 
-def EtaSubst {Γ} {Δ} (sub1 sub2 : Subst Γ Δ) : Type :=
+def EtaSubst {Γ} {Δ} (sub1 sub2 : Subst Γ Δ) : Prop :=
   {x : Var Γ} → closure StepEta (sub1 x) (sub2 x)
 
 theorem closureEtaRename {Γ} {M M' : Term Γ}
@@ -898,23 +870,20 @@ theorem etaProperty {Γ} : square (@StepEta Γ) (@StepEta Γ)
     let ⟨u, bla1, bla2⟩ := etaProperty s1 s2
     ⟨app u _, liftRef (fun x => app x _) StepEta.app1 bla1, liftRef (fun x => app x _) StepEta.app1 bla2⟩
   | StepEta.app1 s1, StepEta.app2 s2 =>
-    ⟨_, Sum.inr (StepEta.app2 s2), Sum.inr (StepEta.app1 s1)⟩
+    ⟨_, Or.inr (StepEta.app2 s2), Or.inr (StepEta.app1 s1)⟩
   | StepEta.app2 s1, StepEta.app1 s2 => -- REPEATED CASE
-    ⟨_, Sum.inr (StepEta.app1 s2), Sum.inr (StepEta.app2 s1)⟩
+    ⟨_, Or.inr (StepEta.app1 s2), Or.inr (StepEta.app2 s1)⟩
   | StepEta.app2 s1, StepEta.app2 s2 =>
     let ⟨u, bla1, bla2⟩ := etaProperty s1 s2
     ⟨app _ u, liftRef (app _) StepEta.app2 bla1, liftRef (app _) StepEta.app2 bla2⟩
   | StepEta.lam s1, StepEta.lam s2 =>
     let ⟨u, bla1, bla2⟩ := etaProperty s1 s2
     ⟨lam u, liftRef lam StepEta.lam bla1, liftRef lam StepEta.lam bla2⟩
-  | StepEta.eta zf1, StepEta.eta zf2 => ⟨_, Sum.inl (Proof.proof rfl), Sum.inl (Proof.proof rfl)⟩
+  | StepEta.eta zf1, StepEta.eta zf2 => ⟨_, Or.inl rfl, Or.inl rfl⟩
   | StepEta.lam (StepEta.app1 s), StepEta.eta zf =>
-    ⟨_, Sum.inr (StepEta.eta (stepEtaZFree s zf)), Sum.inr (substEta s)⟩
+    ⟨_, Or.inr (StepEta.eta (stepEtaZFree s zf)), Or.inr (substEta s)⟩
   | StepEta.eta zf, StepEta.lam (StepEta.app1 s) => -- REPEATED CASE
-    ⟨_, Sum.inr (substEta s), Sum.inr (StepEta.eta (stepEtaZFree s zf))⟩
--- theorem etaDiamond {Γ} {t t1 t2 : Term Γ}
---   (p1 : StepEta t t1) (p2 : StepEta t t2)
---   : Σ t', StepEta t1 t' × StepEta t2 t' :=
+    ⟨_, Or.inr (substEta s), Or.inr (StepEta.eta (stepEtaZFree s zf))⟩
 
 theorem betaEtaCommuteProperty {Γ}
   : square (@Step Γ) (@StepEta Γ) (closure (@StepEta Γ)) (closeRef (@Step Γ)) :=
@@ -934,20 +903,20 @@ theorem betaEtaCommuteProperty {Γ}
         liftRef lam Step.lam q2⟩
     | Step.app1 p1, StepEta.app2 p2 =>
       ⟨_, oneStep (StepEta.app2 p2),
-        Sum.inr (Step.app1 p1)⟩
+        Or.inr (Step.app1 p1)⟩
     | Step.app2 p1, StepEta.app1 p2 => -- REPEATED CASE
       ⟨_, oneStep (StepEta.app1 p2)
-          , Sum.inr (Step.app2 p1)⟩
-    | Step.beta, StepEta.app2 p => ⟨_, subEta closure.refl (oneStep p), Sum.inr Step.beta⟩
-    | Step.beta, StepEta.app1 (StepEta.lam p) => ⟨_, subEta (oneStep p) closure.refl, Sum.inr Step.beta⟩
+          , Or.inr (Step.app2 p1)⟩
+    | Step.beta, StepEta.app2 p => ⟨_, subEta closure.refl (oneStep p), Or.inr Step.beta⟩
+    | Step.beta, StepEta.app1 (StepEta.lam p) => ⟨_, subEta (oneStep p) closure.refl, Or.inr Step.beta⟩
     | Step.beta, StepEta.app1 (StepEta.eta zf) => ⟨_, closure.refl, (by
         rw [subLastZFree (d1 := dummy)]
-        apply Sum.inl (Proof.proof rfl)
+        apply Or.inl rfl
         apply zf
         )⟩
-    | Step.lam (Step.app1 p), StepEta.eta zf => ⟨_, oneStep (StepEta.eta (stepZFree p zf)), Sum.inr (substStep p)⟩
+    | Step.lam (Step.app1 p), StepEta.eta zf => ⟨_, oneStep (StepEta.eta (stepZFree p zf)), Or.inr (substStep p)⟩
     | Step.lam Step.beta, @StepEta.eta _ (lam a) zf =>
-      ⟨_, closure.refl, Sum.inl (Proof.proof (by
+      ⟨_, closure.refl, Or.inl (by
         --
         apply Exists.elim; apply (Iff.mpr lamRenFree zf); intro t proof
         -- rw [<- proof]
@@ -962,7 +931,7 @@ theorem betaEtaCommuteProperty {Γ}
         | Var.zero => rfl
         | Var.succ Var.zero => rfl
         | Var.succ (Var.succ x') => rfl
-        )))⟩
+        ))⟩
 
 --------------------------------------------------------------------------------
 ---------- Equivalence between Par and Step ------------------------------------
@@ -1010,7 +979,7 @@ theorem diamondToProperty {A} {R : Relation A}
   : square R R (closure R) (closeRef R) :=
   fun s1 s2 =>
     let ⟨_, s2', s1'⟩ := d s1 s2
-    ⟨_, oneStep s2', Sum.inr s1'⟩
+    ⟨_, oneStep s2', Or.inr s1'⟩
 theorem parConfluent {Γ} : confluent (@Par Γ) :=
   commutationLemma (diamondToProperty parDiamond)
 theorem stepConfluent {Γ} : confluent (@Step Γ) :=
@@ -1022,8 +991,8 @@ theorem closeRefToClosure {A} {R : Relation A}
   {x y}
   (r : closeRef R x y) : closure R x y :=
   match r with
-  | Sum.inl (Proof.proof rfl) => closure.refl
-  | Sum.inr r => oneStep r
+  | Or.inl rfl => closure.refl
+  | Or.inr r => oneStep r
 
 theorem propertyToProperty {A} {R : Relation A}
   (sq : square R R (closeRef R) (closeRef R))
@@ -1037,300 +1006,5 @@ theorem etaConfluent {Γ} : confluent (@StepEta Γ) :=
 
 def AllStep {Γ} : Relation (Term Γ) := closure (union Step StepEta)
 
-theorem allStepConfluence {Γ} : confluent (union (@Step Γ) StepEta) :=
+theorem confluence {Γ} : confluent (union (@Step Γ) StepEta) :=
   commutativeUnion stepConfluent etaConfluent (commutationLemma betaEtaCommuteProperty)
-
-theorem substUnion1 {n1 n2} {t1 t2 : Term n1} {sub : Subst n1 n2}
-  (rt : AllStep t1 t2)
-  : AllStep (subst sub t1) (subst sub t2) :=
-  match rt with
-  | closure.refl => closure.refl
-  | closure.cons s ss => match s with
-    | union.r beta => closure.cons (union.r (substStep beta)) (substUnion1 ss)
-    | union.s eta => closure.cons (union.s (substEta eta)) (substUnion1 ss)
-
-theorem substUnion2 {n1 n2} {t : Term n1} {sub1 sub2 : Subst n1 n2}
-  (rsub : (x : Var n1) → AllStep (sub1 x) (sub2 x))
-  : AllStep (subst sub1 t) (subst sub2 t) :=
-  match t with
-  | var i => _
-  | app t1 t2 => _
-  | lam t =>
-    _
-
-theorem substUnion {n1 n2} {t1 t2 : Term n1} {sub1 sub2 : Subst n1 n2}
-  (rt : AllStep t1 t2) (rsub : (x : Var n1) → AllStep (sub1 x) (sub2 x))
-  : AllStep (subst sub1 t1) (subst sub2 t2) :=
-  _
-
---------------------------------------------------------------------------------
----------- Making a nicer step relation with a cleaner definition --------------
---------------------------------------------------------------------------------
-
-theorem AllStepZFree {n1 n2} {a b : Term n2}
-  {ren : Ren n1 n2}
-  (r : AllStep a b) (zf : renFree ren a) : renFree ren b :=
-  match r with
-  | closure.refl => zf
-  | closure.cons s ss => match s with
-    | union.r r => AllStepZFree ss (stepZFree r zf)
-    | union.s s => AllStepZFree ss (stepEtaZFree s zf)
-
-inductive Reduces : ∀{Γ}, Term Γ → Term Γ → Prop
-| lam : ∀{Γ} {N N' : Term (succ Γ)},
-  Reduces N N' → Reduces (lam N) (lam N')
-| app : ∀{Γ}{L L' M M' : Term Γ},
-  Reduces L L' → Reduces M M' → Reduces (app L M) (app L' M')
-| beta : ∀{Γ}{N N' : Term (succ Γ)} {M M' : Term Γ},
-  Reduces N N' → Reduces M M' → Reduces (app (lam N) M) (subLast N' M')
-| trans : ∀{Γ} {a b c : Term Γ},
-  Reduces a b → Reduces b c → Reduces a c
-| refl : ∀{Γ} {M : Term Γ}, Reduces M M
-| eta : ∀{Γ} {M M' : Term (succ Γ)},
-  zFree M
-  → Reduces M M'
-  → Reduces (lam (app M (var Var.zero))) (subLast M' dummy)
-
-theorem unionToReduces {Γ} {a b : Term Γ}
-  (steps : AllStep a b) : Reduces a b :=
-  let rec stepToReduces {Γ} {a b : Term Γ}
-  (step : union Step StepEta a b) : Reduces a b :=
-    match step with
-    | union.r beta => match beta with
-      | Step.app1 s => Reduces.app (stepToReduces (union.r s)) Reduces.refl
-      | Step.app2 s => Reduces.app Reduces.refl (stepToReduces (union.r s))
-      | Step.lam s => Reduces.lam (stepToReduces (union.r s))
-      | Step.beta => Reduces.beta Reduces.refl Reduces.refl
-    | union.s eta => match eta with
-      | StepEta.app1 s => Reduces.app (stepToReduces (union.s s)) Reduces.refl
-      | StepEta.app2 s => Reduces.app Reduces.refl (stepToReduces (union.s s))
-      | StepEta.lam s => Reduces.lam (stepToReduces (union.s s))
-      | StepEta.eta zf => Reduces.eta zf Reduces.refl
-  match steps with
-  | closure.refl => Reduces.refl
-  | closure.cons s ss => Reduces.trans (stepToReduces s) (unionToReduces ss)
-
-inductive TypeInhabited (P : Type n) : Prop
-| elem : P → TypeInhabited P
-
-open TypeInhabited
-
-def TIbind {A B : Type n} :
-  TypeInhabited A → (A → TypeInhabited B) → TypeInhabited B :=
-  fun (elem a) f => f a
-
-theorem reducesToUnion {Γ} {a b : Term Γ}
-  (s : Reduces a b) : TypeInhabited (AllStep a b) := by
-  induction s with
-  | lam _r ih => exact (TIbind ih fun a =>
-    elem (liftCsr lam (liftUnion lam Step.lam StepEta.lam) a))
-  | app _r1 _r2 ih1 ih2 => exact (
-    TIbind ih1 fun a =>
-    TIbind ih2 fun b =>
-    elem (
-      transitivity (liftCsr (fun x => app x _) (liftUnion (fun x => app x _) Step.app1 StepEta.app1) a)
-      (liftCsr (app _) (liftUnion (app _) Step.app2 StepEta.app2) b)))
-  | beta _r1 _r2 ih1 ih2 => exact (
-    TIbind ih1 fun a =>
-    TIbind ih2 fun b =>
-    elem (
-      transitivity (liftCsr (fun x => app (lam x) _) (liftUnion _ (Step.app1 ∘ Step.lam) (StepEta.app1 ∘ StepEta.lam)) a)
-      (transitivity (liftCsr (app _) (liftUnion (app _) Step.app2 StepEta.app2) b)
-        (oneStep (union.r Step.beta))
-      )))
-  | eta zf _r ih => exact (TIbind ih fun a =>
-    elem (transitivity
-      (liftCsr (fun x => lam (app x _)) (liftUnion (fun x => lam (app x _)) (Step.lam ∘ Step.app1) (StepEta.lam ∘ StepEta.app1)) a)
-      (oneStep (union.s (StepEta.eta (AllStepZFree a zf))))))
-  | refl => exact (elem closure.refl)
-  | trans _r1 _r2 ih1 ih2 => exact (
-    TIbind ih1 fun a =>
-    TIbind ih2 fun b =>
-    elem (transitivity a b))
-
-
-theorem confluence {Γ} {x y z : Term Γ}
-  : Reduces x y → Reduces x z → ∃ u, Reduces y u ∧ Reduces z u :=
-  fun r s =>
-    let (elem r') := reducesToUnion r
-    let (elem s') := reducesToUnion s
-    let ⟨u, s, t⟩ := allStepConfluence r' s'
-    ⟨u, unionToReduces s, unionToReduces t⟩
-
-def equiv {Γ} : Term Γ → Term Γ → Prop :=
-  fun a b => ∃ c, Reduces a c ∧ Reduces b c
-
-def equivRefl {Γ} {t : Term Γ} : equiv t t := ⟨t, Reduces.refl, Reduces.refl⟩
-
-theorem equivLam {Γ} {a b : Term (succ Γ)}
-  (eq : equiv a b) : equiv (lam a) (lam b) :=
-  let ⟨t, ra, rb⟩ := eq
-  ⟨lam t, Reduces.lam ra, Reduces.lam rb⟩
-
-theorem equivApp {Γ} {a1 b1 a2 b2 : Term Γ}
-  (eq1 : equiv a1 a2) (eq2 : equiv b1 b2)
-  : equiv (app a1 b1) (app a2 b2) :=
-  let ⟨a, ra1, ra2⟩ := eq1
-  let ⟨b, rb1, rb2⟩ := eq2
-  ⟨app a b, Reduces.app ra1 rb1, Reduces.app ra2 rb2⟩
-
-def SubstReduces {n1 n2} (sub1 sub2 : Subst n1 n2) : Prop :=
-  (x : Var n1) → Reduces (sub1 x) (sub2 x)
-
-def SubstEquiv {n1 n2} (sub1 sub2 : Subst n1 n2) : Prop :=
-  ∃ sub, SubstReduces sub1 sub ∧ SubstReduces sub2 sub
-
-def substEquivRefl {n1 n2} {sub : Subst n1 n2} : SubstEquiv sub sub :=
-  ⟨sub, fun _ => Reduces.refl, fun _ => Reduces.refl⟩
-
-theorem reducesSubst {n1 n2} {t1 t2 : Term n1} {sub1 sub2 : Subst n1 n2}
-  (rt : Reduces t1 t2) (rsub : SubstReduces sub1 sub2)
-  : Reduces (subst sub1 t1) (subst sub2 t2) :=
-  (unionToReduces _)
-
-theorem equivSubst {n1 n2} {t1 t2 : Term n1} {sub1 sub2 : Subst n1 n2}
-  (eq1 : equiv t1 t2) (eq2 : SubstEquiv sub1 sub2)
-  : equiv (subst sub1 t1) (subst sub2 t2) :=
-  _
-
-def QTerm (Γ : Context) : Type := Quot (@equiv Γ)
-
-def q {Γ} : Term Γ → QTerm Γ :=
-  fun t => Quot.mk equiv t
-
-def lift {Γ} {β : Sort u}
-  : (f : Term Γ → β)
-    → (∀ {a b}, equiv a b → f a = f b) → Quot (@equiv Γ) → β := Quot.lift
-
-def lift2 {Γ} {β : Sort u}
-  : (f : Term Γ → Term Γ → β)
-    → (∀ {a b a' b'}, equiv a b → equiv a' b' → f a a' = f b b')
-    → Quot (@equiv Γ) → Quot (@equiv Γ) → β :=
-    fun f proof q1 q2 =>
-    lift (fun t1 q2 => lift (fun t2 => f t1 t2) (fun eq => (proof equivRefl eq)) q2)
-      (fun eq => by (
-        apply funext
-        apply Quot.ind
-        simp [lift]
-        intro a
-        apply (proof eq equivRefl)))
-      q1 q2
-
-def qlam {Γ} : QTerm (succ Γ) → QTerm Γ :=
-  fun t => lift (q ∘ lam) (fun eq => (Quot.sound (equivLam eq))) t
-
-theorem qlamWorksDefinitionally {Γ} {t : Term (succ Γ)}
-  : qlam (q t) = q (lam t) := by rfl
-
-
-def qapp {Γ} : QTerm Γ → QTerm Γ → QTerm Γ :=
-  fun a b => lift2 (fun t1 t2 => q (app t1 t2)) (fun eq1 eq2 => Quot.sound (equivApp eq1 eq2)) a b
-
-theorem qappWorksDefinitionally {Γ} {a b : Term Γ}
-  : qapp (q a) (q b) = q (app a b) := rfl
-
-theorem exampleInequality :
-  @ q zero (lam (lam (var Var.zero))) ≠ q (lam (lam (var (Var.succ Var.zero)))) := by
-  intro eq
-  --
-  sorry
-
-def qSubst : Context → Context → Type := fun n1 n2 => Var n1 → QTerm n2
-
--- def substEquiv {n1 n2} (s1 s2 : Subst n1 n2) : Prop := (x : Var n1) → equiv (s1 x) (s2 x)
-
-def qSubst2 : Context → Context → Type := fun n1 n2 => Quot (@SubstEquiv n1 n2)
-
-def qsubst2 {n1 n2} (qsub : qSubst2 n1 n2) (qt : QTerm n1) : QTerm n2 :=
-  Quot.lift (fun sub => lift (fun t => q (subst sub t)) (fun eq => Quot.sound (equivSubst eq substEquivRefl)) qt)
-    (fun _ _ seq => by
-      simp[lift, Quot.lift];
-      apply (Quot.ind (β := fun qt => Quot.lift _ _ qt = Quot.lift _ _ qt) _ qt)
-      simp
-      intro a
-      apply Quot.sound
-      apply equivSubst
-      apply equivRefl
-      apply seq
-    ) qsub
-
-theorem qsubst2app {n1 n2} {qsub : qSubst2 n1 n2} (q1 q2 : QTerm n1)
-  : qsubst2 qsub (qapp q1 q2) = qapp (qsubst2 qsub q1) (qsubst2 qsub q2) := by
-    -- have lemma1 {t1} {q2} : qsubst2 qsub (qapp (q t1) q2) = qapp (qsubst2 qsub (q t1)) (qsubst2 qsub q2) := by
-    --   sorry
-    have lemma {n} {t : Term n} : q t = Quot.mk equiv t := by rfl
-    revert q1
-    apply Quot.ind
-    intro t1
-    revert q2
-    apply Quot.ind
-    intro t2
-    repeat rw [<- lemma]
-    rw [qappWorksDefinitionally]
-    simp [qapp, lift2, lift, Quot.lift]
-    simp [qapp, qsubst2]
-    --
-
--- def subLast {n} (t1 : Term (succ n)) (t2 : Term n) : Term n :=
---   subst (substZero t2) t1
--- def qSubLast {n} (q1 : QTerm (succ n)) (q2 : QTerm n) : QTerm n :=
---   qsubst2 (substZero _) q1
-
-
--- def qSubstTo2 {n1 n2} : qSubst n1 n2 → qSubst2 n1 n2 := fun s =>
---   _
-
-def qexts {n1 n2} (sub : qSubst n1 n2) : qSubst (succ n1) (succ n2) :=
-  fun x => match x with
-           | Var.zero => q (var Var.zero)
-           | Var.succ x' => _ -- rename Var.succ (sub x')
-
-def tsubst {n1 n2} (s : qSubst n1 n2) (t : Term n1) : QTerm n2 :=
-  match t with
-  | var i => s i
-  | lam t => qlam (tsubst (qexts s) t)
-  | app t1 t2 => qapp (tsubst s t1) (tsubst s t2)
-
-def qsubst {n1 n2} (s : qSubst n1 n2) (t : QTerm n1) : QTerm n2 :=
-  lift (tsubst s) _ t
-
--- there has to be a better way. I just proved all that stuff up to confluence, surely I can use it now.
-
-def lift2' {A B} {R : A → A → Prop} {S : B → B → Prop} {β : Sort u}
-  : (f : A → B → β)
-    → (∀ {a b a' b'}, R a b → S a' b' → f a a' = f b b')
-    → Quot R → Quot S → β := sorry
-    -- fun f proof q1 q2 =>
-    -- Quot.lift (fun t1 q2 => Quot.lift (fun t2 => f t1 t2) (fun eq => _) q2)
-    --   (fun eq => by (
-    --     apply funext
-    --     apply Quot.ind
-    --     simp [lift]
-    --     intro a
-    --     apply (proof eq equivRefl)))
-    --   q1 q2
-
--- def qsubst2 {n1 n2} (s : Subst n1 n2) (t : QTerm n1) : QTerm n2 :=
-
--- as an example:
-def qSubLast {n} (q1 : QTerm (succ n)) (q2 : QTerm n) : QTerm n :=
-  lift2' (fun t1 t2 => q (subLast t1 t2)) (fun eq1 eq2 => Quot.sound _) q1 q2
-
-def qBeta : ∀ {Γ} {N : QTerm (succ Γ)} {M : QTerm Γ},
-    (qapp (qlam N) M) = (qSubLast N M) :=
-    _
-
-def wk {n} (qt : QTerm n) : QTerm (succ n) :=
-  lift (fun t => q (rename Var.succ t)) (fun eq => Quot.sound _) qt
-
--- -- An example to try out proving equality by rewriting:
-theorem exampleEquality {M : QTerm zero}
-  : qapp (qlam (wk M)) M = M := by
-  --
-  rw [qBeta]
-  --
-  sorry
-
--- theorem qapp ((qlam t) t2) = t [t2]
-
--- tactic simplify = repeat rw [qapp, ...] at *
