test2025/theorempropositin.lean
@@ -1,0 +1,2 @@
+theorem anumber : Nat := by
+  exact 1
